src/ParametricWf.v
@@ -2,7 +2,7 @@ Require Import Bool List String Structures.Equalities.
 Require Import Lib.Struct Lib.Word Lib.CommonTactics.
 Require Import Lib.StringBound Lib.ilist Lib.FMap Lib.StringEq.
 Require Import Lts.Syntax Lts.SemanticsExprAction Lts.Semantics Lts.Equiv Lts.Wf.
-Require Import Lts.ParametricSyntax.
+Require Import Lts.ParametricSyntax Lib.Indexer.
 Require Import FunctionalExtensionality Program.Equality Eqdep Eqdep_dec.
 
 Set Implicit Arguments.
